examples/bw/BWMain01proof.v
@@ -16,8 +16,8 @@ From ExtLib Require Import
      Structures.Maps
      Data.Map.FMapAList.
 Require Import TODOYJ.
-Require Import Logic YPM.
 Require Import HTactics.
+Require Import Logic YPM.
 
 Generalizable Variables E R A B C X Y.
 
@@ -42,42 +42,7 @@ Lemma unfold_APC: forall n, _APC n =
   { i. destruct n; ss. }
 Qed.
 Global Opaque _APC.
-Ltac harg_tac :=
-  HTactics.harg_tac;
-  match goal with
-  | [H: URA.wf ?cur |- _] =>
-    let name := fresh "GWF" in
-    assert(name: __gwf_mark__ cur cur) by (split; [refl|exact H]); clear H
-  end.
 
-Ltac hcall_tac x o MR_SRC1 FR_SRC1 RARG_SRC :=
-  let mr_src1 := r_gather MR_SRC1 in
-  let fr_src1 := r_gather FR_SRC1 in
-  let rarg_src := r_gather RARG_SRC in
-  (* let tac0 := etrans; [on_gwf ltac:(fun GWF => apply GWF)|eapply URA.extends_updatable; r_equalize; r_solve] in *)
-  (* let tac0 := idtac in *)
-  let tac0 := etrans; [etrans; [|on_gwf ltac:(fun GWF => apply GWF)]|]; eapply URA.extends_updatable; r_equalize; r_solve; fail in
-  let tac1 := (on_gwf ltac:(fun H => clear H);
-               let WF := fresh "WF" in
-               let tmp := fresh "_tmp_" in
-               let GWF := fresh "GWF" in
-               intros ? ? ? ? ? WF; cbn in WF; desH WF; subst;
-               esplits; ss; et; intros tmp ?; assert(GWF: ☀) by (split; [refl|exact tmp]); clear tmp; iRefresh; iClears') in
-  prep;
-  match x with
-  | ltac_wild =>
-    match o with
-    | ltac_wild => eapply (hcall_clo _ (mr_src1:=mr_src1) (fr_src1:=fr_src1) (rarg_src:=rarg_src)); [tac0|lia|..|tac1]
-    | _ => eapply (hcall_clo _ (o:=o) (mr_src1:=mr_src1) (fr_src1:=fr_src1) (rarg_src:=rarg_src)); [tac0|lia|..|tac1]
-    end
-  | _ => eapply (hcall_clo x (o:=o) (mr_src1:=mr_src1) (fr_src1:=fr_src1) (rarg_src:=rarg_src)); [tac0|lia|..|tac1]
-  end
-.
-Ltac hret_tac MR_SRC RT_SRC :=
-  let mr_src1 := r_gather MR_SRC in
-  let fr_src1 := r_gather RT_SRC in
-  HTactics.hret_tac mr_src1 fr_src1
-.
 
 
 Section SIMMODSEM.
