mem/Mem02proof.v
@@ -1,0 +1,777 @@
+Require Import Mem0 Mem1 Mem2 HoareDef SimModSem.
+Require Import Coqlib.
+Require Import Universe.
+Require Import Skeleton.
+Require Import PCM.
+Require Import ModSem Behavior.
+Require Import Relation_Definitions.
+
+(*** TODO: export these in Coqlib or Universe ***)
+Require Import Relation_Operators.
+Require Import RelationPairs.
+From ITree Require Import
+     Events.MapDefault.
+From ExtLib Require Import
+     Core.RelDec
+     Structures.Maps
+     Data.Map.FMapAList.
+Require Import TODOYJ.
+Require Import HTactics Logic YPM.
+
+Generalizable Variables E R A B C X Y.
+
+Set Implicit Arguments.
+
+Local Open Scope nat_scope.
+
+
+
+(*** black + delta --> new_black ***)
+Definition add_delta_to_black `{M: URA.t} (b: URA.auth_t) (w: URA.auth_t): URA.auth_t :=
+  match b, w with
+  | URA.excl e _, URA.frag f1 => URA.excl (URA.add e f1) URA.unit
+  | _, _ => URA.boom
+  end
+.
+
+
+(* Notation "wf n *)
+(* '------------------------------------------------------------------' *)
+(* src0 tgt0 *)
+(* '------------------------------------------------------------------' *)
+(* src1 tgt1 *)
+(* '------------------------------------------------------------------' *)
+(* src2 tgt2" := *)
+(*   (sim_itree wf n (([(_, src0)], src1), src2) (([(_, tgt0)], tgt1), tgt2)) *)
+(*     (at level 60, *)
+(*      format "wf  n '//' *)
+(* '------------------------------------------------------------------' '//' *)
+(* src0 '//' *)
+(* tgt0 '//' *)
+(* '------------------------------------------------------------------' '//' *)
+(* src1 '//' *)
+(* tgt1 '//' *)
+(* '------------------------------------------------------------------' '//' *)
+(* src2 '//' '//' '//' *)
+(* tgt2 '//' *)
+(* "). *)
+(******** TODO: it works in emacs but fails in coqc -- try coq 8.13 and uncomment it ***********)
+
+Lemma repeat_nth_some
+      X (x: X) sz ofs
+      (IN: ofs < sz)
+  :
+    nth_error (repeat x sz) ofs = Some x
+.
+Proof.
+  ginduction sz; ii; ss.
+  - lia.
+  - destruct ofs; ss. exploit IHsz; et. lia.
+Qed.
+
+Lemma repeat_nth_none
+      X (x: X) sz ofs
+      (IN: ~(ofs < sz))
+  :
+    nth_error (repeat x sz) ofs = None
+.
+Proof.
+  generalize dependent ofs. induction sz; ii; ss.
+  - destruct ofs; ss.
+  - destruct ofs; ss. { lia. } hexploit (IHsz ofs); et. lia.
+Qed.
+
+Lemma repeat_nth
+      X (x: X) sz ofs
+  :
+    nth_error (repeat x sz) ofs = if (ofs <? sz) then Some x else None
+.
+Proof.
+  des_ifs.
+  - eapply repeat_nth_some; et. apply_all_once Nat.ltb_lt. ss.
+  - eapply repeat_nth_none; et. apply_all_once Nat.ltb_ge. lia.
+Qed.
+
+
+
+Section AUX.
+  Context `{Σ: GRA.t}.
+  Definition Univ {X: Type} (P: X -> iProp): iProp := fun r => forall x, P x r.
+End AUX.
+Notation "'Forall' x .. y , p" := (Univ (fun x => .. (Univ (fun y => p)) ..))
+                                    (at level 200, x binder, right associativity,
+                                     format "'[' 'Forall'  '/  ' x  ..  y ,  '/  ' p ']'").
+
+
+Section SIMMODSEM.
+
+  Context `{Σ: GRA.t}.
+  Context `{@GRA.inG Mem1.memRA Σ}.
+
+
+  Definition _points_to (loc: block * Z) (vs: list val): Mem1._memRA :=
+    let (b, ofs) := loc in
+    (fun _b _ofs => if (dec _b b) && ((ofs <=? _ofs) && (_ofs <? (ofs + Z.of_nat (List.length vs))))%Z
+                    then inl (List.nth_error vs (Z.to_nat (_ofs - ofs))) else inr tt)
+  .
+
+
+
+  Let W: Type := (alist mname (Σ * Any.t)) * (alist mname (Σ * Any.t)).
+  (* Eval compute in (@RA.car (RA.excl Mem.t)). *)
+  Eval compute in (@URA.car Mem1._memRA).
+  Inductive sim_loc: option val -> (option val + unit) -> Prop :=
+  | sim_loc_present v: sim_loc (Some v) (inl (Some v))
+  | sim_loc_absent: sim_loc None (inr tt)
+  .
+
+  Let wf: W -> Prop :=
+    fun '(mrps_src0, mrps_tgt0) =>
+      exists mr_src (mem_tgt: Mem.t),
+        (<<SRC: mrps_src0 = Maps.add "Mem" (mr_src, tt↑) Maps.empty>>) /\
+        (<<TGT: mrps_tgt0 = Maps.add "Mem" (ε, mem_tgt↑) Maps.empty>>) /\
+        (* (<<SIM: forall b ofs, sim_loc ((mem_tgt.(Mem.cnts)) b ofs) (mem_src b ofs)>>) *)
+        (* (<<SIM: forall b ofs v, (mem_tgt.(Mem.cnts) b ofs = Some v) -> iHyp (⌜True⌝) mem_src>>) *)
+        (* (<<SIM: iHyp (Forall b ofs v, ⌜mem_tgt.(Mem.cnts) b ofs = Some v⌝ -* Own (GRA.embed ((b, ofs) |-> [v]))) mem_src>>) *)
+        (<<SIM: iHyp (Exists mem_src, Own (GRA.embed ((URA.black mem_src): URA.car (t:=Mem1.memRA))) **
+                                          (* (Forall b ofs, ⌜~(b = 0 /\ ofs = 0%Z)⌝ -* *)
+                                          (*                  match mem_tgt.(Mem.cnts) b ofs with *)
+                                          (*                  | Some v => Own (GRA.embed ((b, ofs) |-> [v])) *)
+                                          (*                  | None => ⌜True⌝ *)
+                                          (*                  end) *)
+                                          (⌜forall b ofs, sim_loc ((mem_tgt.(Mem.cnts)) b ofs) (mem_src b ofs)⌝)
+                     ) mr_src>>) /\
+        (<<WFTGT: forall b ofs v, mem_tgt.(Mem.cnts) b ofs = Some v -> <<NB: b < mem_tgt.(Mem.nb)>> >>)
+  .
+
+  Local Opaque points_to.
+
+  Hint Resolve sim_itree_mon: paco.
+
+  Opaque URA.unit.
+
+  Theorem correct: ModSemPair.sim Mem2.MemSem Mem0.MemSem.
+  Proof.
+   econstructor 1 with (wf:=wf) (le:=top2); et; swap 2 3.
+    { typeclasses eauto. }
+    { ss. esplits; ss; et. hexploit gwf_dummy; i. iRefresh.
+      eexists; iRefresh. iSplitP; ss.
+      { eexists. rewrite URA.unit_id. refl. }
+      ii. econs.
+    }
+
+    econs; ss.
+    { unfold allocF. init.
+      harg_tac. des_ifs_safe. des. repeat rewrite URA.unit_idl in *. repeat rewrite URA.unit_id in *.
+      iRefresh. iPure PRE. des. clarify. apply Any.upcast_inj in PRE. des; clarify.
+      steps. rewrite Any.upcast_downcast in *. steps.
+      do 2 iDestruct SIM. iPure A.
+      set (blk := (Mem.nb mem_tgt)). rename x into sz. rename x0 into mem_src0.
+
+      unfold interp_hCallE_tgt, APC. steps. (********** TODO: never unfold it, make a lemma ******************)
+      force_l. exists 0. steps.
+
+      eapply own_upd in SIM; cycle 1; [|rewrite intro_iHyp in SIM; iMod SIM].
+      { eapply GRA.embed_updatable.
+        eapply URA.auth_alloc2.
+        instantiate (1:=(_points_to (blk, 0%Z) (repeat (Vint 0) sz))).
+        (* instantiate (1:=(fun _b _ofs => if (dec _b blk) && ((0 <=? _ofs) && (_ofs <? Z.of_nat sz))%Z then inl (Some (Vint 0)) else inr tt)). *)
+        iOwnWf SIM. iRefresh.
+        clear - WF WFTGT A.
+        ss. ii. des_ifs.
+         - bsimpl. des. des_sumbool. subst. hexploit (A blk k0); et. intro T. inv T; [|eq_closure_tac].
+           exploit WFTGT; et. i; des. lia.
+         - specialize (A k k0). inv A; eq_closure_tac.
+         - rewrite Z.sub_0_r. bsimpl. des. des_sumbool. subst. apply_all_once Z.leb_le. apply_all_once Z.ltb_lt.
+           intro B. apply nth_error_None in B. lia.
+      }
+      rewrite <- GRA.embed_add in SIM. rewrite own_sep in SIM. iDestruct SIM.
+
+      force_l. eexists. hret_tac SIM A0.
+      - split; [|refl]; iRefresh. eexists; iRefresh. iSplitP; ss.
+      - cbn. esplits; et.
+        + eexists; iRefresh. iSplitL SIM; et. ii.
+          destruct (mem_tgt.(Mem.cnts) blk ofs) eqn:T.
+          { exfalso. exploit WFTGT; et. i; des. lia. }
+          exploit A; et. rewrite T. intro U. inv U. ss. rewrite repeat_length.
+          destruct (dec b blk).
+          * subst. ss. unfold update. des_ifs_safe. des_ifs.
+            { rewrite Z.sub_0_r. bsimpl. des. apply_all_once Z.leb_le. apply_all_once Z.ltb_lt.
+              rewrite repeat_nth_some; try lia. econs. }
+            { econs. }
+          * ss. unfold update. des_ifs_safe.
+            hexploit (A b ofs); et. intro V. inv V; ss.
+            { econs. }
+            { econs. }
+        + clear - WFTGT. i. ss. unfold update in *. des_ifs. exploit WFTGT; et.
+    }
+    econs; ss.
+    { unfold freeF. init.
+      harg_tac. des_ifs_safe. des. repeat rewrite URA.unit_idl in *. repeat rewrite URA.unit_id in *.
+      iRefresh. do 3 iDestruct PRE. iPure PRE. iPure A. clarify. apply Any.upcast_inj in PRE. des; clarify.
+      do 2 iDestruct SIM. iPure A.
+      steps. rewrite Any.upcast_downcast in *. steps.
+
+      unfold interp_hCallE_tgt, APC. steps. (********** TODO: never unfold it, make a lemma ******************)
+      force_l. exists 0. steps.
+
+      rename n into b. rename z into ofs. rename x0 into mem_src0. rename x into v.
+      iMerge SIM A0. rewrite <- own_sep in SIM. rewrite GRA.embed_add in SIM.
+      iOwnWf SIM. eapply GRA.embed_wf in WF; des.
+      assert(HIT: mem_src0 b ofs = inl (Some v)).
+      { clear - WF.
+        Local Transparent points_to.
+        (* assert(A: mem_src0 b ofs <> inl None). *)
+        (* { ss. des. admit "". } *)
+        dup WF. rename WF0 into X.
+        eapply URA.auth_included in WF.
+        ss. des. rr in WF. des. subst. ss.
+        destruct (dec b b); ss. destruct (ofs <=? ofs)%Z eqn:T; ss; cycle 1.
+        { try rewrite Z.leb_le in *; try rewrite Z.leb_gt in *; try rewrite Z.ltb_lt in *; try rewrite Z.ltb_ge in *; try lia. }
+        destruct ((ofs <? ofs + 1)%Z) eqn:U; ss; cycle 1.
+        { try rewrite Z.leb_le in *; try rewrite Z.leb_gt in *; try rewrite Z.ltb_lt in *; try rewrite Z.ltb_ge in *; try lia. }
+        destruct (ctx b ofs) eqn:V; ss; cycle 1.
+        { try rewrite Z.sub_diag in *. ss. }
+        specialize (X0 b ofs). des_ifs_safe. clear - Heq1. bsimpl. des_sumbool; ss.
+      }
+      set (mem_src1 := fun _b _ofs => if dec _b b && dec _ofs ofs then inr () else mem_src0 _b _ofs).
+      assert(WF': URA.wf (mem_src1: URA.car (t:=Mem1._memRA))).
+      { unfold mem_src1. ss. ii. des_ifs. des. exploit WF0; et. rewrite Heq. ii; ss. }
+      hexploit (A b ofs); et. rewrite HIT. intro B. inv B.
+      force_r.
+      { unfold Mem.free in *. des_ifs. }
+      rename mem_tgt into mem_tgt0. rename t into mem_tgt1.
+
+      eapply own_upd in SIM; cycle 1; [|rewrite intro_iHyp in SIM; iMod SIM].
+      { eapply GRA.embed_updatable.
+        Local Transparent points_to.
+        eapply URA.auth_dealloc.
+        instantiate (1:=mem_src1).
+        clear - WF'.
+
+        r. i. rewrite URA.unit_idl.
+        Local Opaque Mem1._memRA.
+        ss. destruct H; clear H. (*** coq bug; des infloops ***) des. clarify.
+        esplits; et.
+        Local Transparent Mem1._memRA.
+        apply func_ext. intro _b. apply func_ext. intro _ofs.
+        destruct (classic (b = _b /\ ofs = _ofs)).
+        - destruct H; clear H. clarify.
+          subst mem_src1. ss. des_ifs; bsimpl; des; des_sumbool; clarify.
+          clear - H0.
+          Local Transparent URA.wf.
+          Local Transparent URA.add.
+          specialize (H0 _b _ofs). ss.
+          des_ifs; bsimpl; des; des_sumbool;
+            try rewrite Z.leb_le in *; try rewrite Z.leb_gt in *; try rewrite Z.ltb_lt in *; try rewrite Z.ltb_ge in *;
+              try rewrite Z.sub_diag in *;
+              try lia; ss.
+          des_u. ss.
+        - Psimpl.
+          subst mem_src1. s.
+          des_ifs; bsimpl; des; des_sumbool;
+            try rewrite Z.leb_le in *; try rewrite Z.leb_gt in *; try rewrite Z.ltb_lt in *; try rewrite Z.ltb_ge in *;
+              try rewrite Z.sub_diag in *;
+              try lia; ss.
+          Local Opaque URA.wf.
+          Local Opaque URA.add.
+      }
+      steps. iRefresh. force_l. eexists. hret_tac SIM (@URA.unit Σ).
+      { split; [|refl]. ss. }
+      { ss. esplits; ss; et.
+        - eexists mem_src1; iRefresh. iSplitP; ss. ii.
+          { unfold Mem.free in _UNWRAPU. des_ifs. ss.
+            subst mem_src1. ss.
+            destruct (classic (b = b0 /\ ofs = ofs0)); des; clarify.
+            - unfold update. des_ifs. econs.
+            - des_ifs.
+              { Psimpl. bsimpl; des; des_sumbool; ss; clarify. }
+              replace (update (Mem.cnts mem_tgt0) b (update (Mem.cnts mem_tgt0 b) ofs None) b0 ofs0) with
+                  (Mem.cnts mem_tgt0 b0 ofs0); cycle 1.
+              { unfold update. des_ifs. Psimpl. des_ifs; bsimpl; des; des_sumbool; ss; clarify. }
+              et.
+          }
+        - clear - _UNWRAPU WFTGT. ii. unfold Mem.free in *. des_ifs. ss.
+          unfold update in *. des_ifs; eapply WFTGT; et.
+      }
+    }
+    econs; ss.
+    { unfold loadF. init.
+      harg_tac. des_ifs_safe. des. repeat rewrite URA.unit_idl in *. repeat rewrite URA.unit_id in *.
+      iRefresh. do 2 iDestruct PRE. iPure PRE. iPure A. clarify. apply Any.upcast_inj in PRE. des; clarify.
+      do 2 iDestruct SIM. iPure A.
+      steps. rewrite Any.upcast_downcast in *. steps.
+
+      unfold interp_hCallE_tgt, APC. steps. (********** TODO: never unfold it, make a lemma ******************)
+      force_l. exists 0. steps.
+      rename n into b. rename z into ofs. rename x into mem_src0.
+      iMerge SIM A0. rewrite <- own_sep in SIM. rewrite GRA.embed_add in SIM. iOwnWf SIM.
+      assert(T: mem_src0 b ofs = inl (Some v)).
+      { clear - WF.
+        apply GRA.embed_wf in WF. des; ss.
+        Local Transparent points_to URA.add URA.wf.
+        ss. des. do 2 spc WF0. rr in WF. des. ss.
+        des_ifs; bsimpl; des; des_sumbool; ss;
+          try rewrite Z.leb_le in *; try rewrite Z.leb_gt in *; try rewrite Z.ltb_lt in *; try rewrite Z.ltb_ge in *;
+            try rewrite Z.sub_diag in *; try lia; ss.
+        Local Opaque points_to URA.add URA.wf.
+      }
+      exploit A; et. intro U. rewrite T in U. inv U; ss. unfold Mem.load.
+      rewrite <- GRA.embed_add in SIM. rewrite own_sep in SIM. iDestruct SIM.
+      force_r; ss. clarify. steps. force_l. esplits.
+      hret_tac SIM A0.
+      { split; [|refl]; iRefresh. iSplitP; ss. }
+      { ss. esplits; eauto. eexists; iRefresh. iSplitP; ss; et. }
+    }
+    econs; ss.
+    { unfold storeF. init.
+      harg_tac. des_ifs_safe. des. repeat rewrite URA.unit_idl in *. repeat rewrite URA.unit_id in *.
+      iRefresh. do 3 iDestruct PRE. iPure PRE. iPure A. clarify. apply Any.upcast_inj in PRE. des; clarify.
+      do 2 iDestruct SIM. iPure A.
+      steps. rewrite Any.upcast_downcast in *. steps.
+
+      unfold interp_hCallE_tgt, APC. steps. (********** TODO: never unfold it, make a lemma ******************)
+      force_l. exists 0. steps.
+      rename n into b. rename z into ofs. rename x into mem_src0.
+      iMerge SIM A0. rewrite <- own_sep in SIM. rewrite GRA.embed_add in SIM. iOwnWf SIM.
+      assert(T: mem_src0 b ofs = inl (Some v)).
+      { clear - WF.
+        apply GRA.embed_wf in WF. des; ss.
+        Local Transparent points_to URA.add URA.wf.
+        ss. des. do 2 spc WF0. rr in WF. des. ss.
+        des_ifs; bsimpl; des; des_sumbool; ss;
+          try rewrite Z.leb_le in *; try rewrite Z.leb_gt in *; try rewrite Z.ltb_lt in *; try rewrite Z.ltb_ge in *;
+            try rewrite Z.sub_diag in *; try lia; ss.
+        Local Opaque points_to URA.add URA.wf.
+      }
+      exploit A; et. intro U. rewrite T in U. inv U; ss. unfold Mem.load.
+      rewrite <- GRA.embed_add in SIM. rewrite own_sep in SIM. iDestruct SIM.
+      force_r; ss. clarify. steps. force_l. esplits.
+      hret_tac SIM A0.
+      { split; [|refl]; iRefresh. iSplitP; ss. }
+      { ss. esplits; eauto. eexists; iRefresh. iSplitP; ss; et. }
+    }
+    { unfold loadF. init. harg_tac. des; clarify.
+      unfold interp_hCallE_tgt, APC. steps. anytac. ss.
+      steps. force_l. exists 0. steps. anytac. ss. steps.
+      rewrite URA.unit_idl in *. rewrite GRA.embed_add in *. apply_all_once GRA.embed_wf. des.
+      rename n into b. rename z into ofs.
+      assert(T: mem_src b ofs = inl (Some v)).
+      { Local Transparent points_to URA.add URA.wf URA.unit.
+        clear - VALID.
+        ss. des. do 2 spc VALID0. rr in VALID. des. ss.
+        des_ifs; bsimpl; des; des_sumbool; ss;
+          try rewrite Z.leb_le in *; try rewrite Z.leb_gt in *; try rewrite Z.ltb_lt in *; try rewrite Z.ltb_ge in *;
+            try rewrite Z.sub_diag in *; try lia; ss.
+        Local Opaque points_to URA.add URA.wf URA.unit.
+      }
+      exploit SIM; et. intro U. rewrite T in U. inv U; ss. unfold Mem.load.
+      force_r; ss. clarify. steps. force_l. esplits.
+      hret_tac (GRA.embed (URA.black (mem_src: URA.car (t:=Mem1._memRA)))) (GRA.embed ((b, ofs) |-> [v0])); ss.
+      esplits; eauto.
+    }
+
+
+    steps. iRefresh. force_l. eexists. hret_tac
+
+
+
+
+      assert(SIM': forall b ofs, sim_loc (Mem.cnts mem_tgt' b ofs) (mem_src' b ofs)).
+      { i.
+        unfold Mem.free in _UNWRAPU. des_ifs. ss.
+        subst mem_src'. ss.
+        destruct (classic (b = b0 /\ ofs = ofs0)); des; clarify.
+        - destruct H0; clarify. (**** TODO: FIX ****) unfold update. des_ifs. econs.
+        - des_ifs.
+          { Psimpl. bsimpl; des; des_sumbool; ss; clarify. destruct H0; ss. destruct H1; ss. (**** TODO: FIX ****)}
+          replace (update (Mem.cnts mem_tgt) b (update (Mem.cnts mem_tgt b) ofs None) b0 ofs0) with
+              (Mem.cnts mem_tgt b0 ofs0); cycle 1.
+          { unfold update. des_ifs. Psimpl. des_ifs; bsimpl; des; des_sumbool; ss; clarify. }
+          et.
+      }
+
+      iMerge SIM A0. rewrite <- own_sep in SIM. rewrite GRA.embed_add in SIM.
+      eapply own_upd in SIM; cycle 1; [|rewrite intro_iHyp in SIM; iMod SIM].
+      { eapply GRA.embed_updatable.
+        Local Transparent points_to.
+        eapply URA.auth_dealloc.
+        Local Opaque points_to.
+
+
+        instantiate (1:=(_points_to (blk, 0%Z) (repeat (Vint 0) sz))).
+        (* instantiate (1:=(fun _b _ofs => if (dec _b blk) && ((0 <=? _ofs) && (_ofs <? Z.of_nat sz))%Z then inl (Some (Vint 0)) else inr tt)). *)
+        iOwnWf SIM. iRefresh.
+        clear - WF WFTGT A.
+        ss. ii. des_ifs.
+         - bsimpl. des. des_sumbool. subst. hexploit (A blk k0); et. intro T. inv T; [|eq_closure_tac].
+           exploit WFTGT; et. i; des. lia.
+         - specialize (A k k0). inv A; eq_closure_tac.
+         - rewrite Z.sub_0_r. bsimpl. des. des_sumbool. subst. apply_all_once Z.leb_le. apply_all_once Z.ltb_lt.
+           intro B. apply nth_error_None in B. lia.
+      }
+      rewrite <- GRA.embed_add in SIM. rewrite own_sep in SIM. iDestruct SIM.
+
+      force_l. eexists. hret_tac SIM A0.
+      - split; [|refl]; iRefresh. eexists; iRefresh. iSplitP; ss.
+      - cbn. esplits; et.
+        + eexists; iRefresh. iSplitL SIM; et. ii.
+          destruct (mem_tgt.(Mem.cnts) blk ofs) eqn:T.
+          { exfalso. exploit WFTGT; et. i; des. lia. }
+          exploit A; et. rewrite T. intro U. inv U. ss. rewrite repeat_length.
+          destruct (dec b blk).
+          * subst. ss. unfold update. des_ifs_safe. des_ifs.
+            { rewrite Z.sub_0_r. bsimpl. des. apply_all_once Z.leb_le. apply_all_once Z.ltb_lt.
+              rewrite repeat_nth_some; try lia. econs. }
+            { econs. }
+          * ss. unfold update. des_ifs_safe.
+            hexploit (A b ofs); et. intro V. inv V; ss.
+            { econs. }
+            { econs. }
+        + clear - WFTGT. i. ss. unfold update in *. des_ifs. exploit WFTGT; et.
+    }
+            des_ifs.
+            { eq_closure_tac. }
+          * ss.
+            destruct (mem_src0 blk ofs) eqn:U.
+            {
+            assert(mem_tgt.(Mem.cnts) blk ofs = None).
+            {
+        +
+             exploit A; et. bsimpl. des. des_sumbool. subst. hexploit (A blk k0); et. intro T. inv T; [|eq_closure_tac].
+           exploit WFTGT; et. i; des. lia.
+         -
+           clear - H1. subst blk. ss.
+           apply_all_once Z.leb_le. apply_all_once Z.ltb_lt.
+           bsimpl; des; des_sumbool; ss.
+        instantiate(1:=(fun _b _ofs => if (dec _b b) && ((ofs <=? _ofs) && (_ofs <? (ofs + Z.of_nat (List.length (List.repeat 0 sz)))))%Z
+                              then inl (List.nth_error (List.repeat 0 sz) (Z.to_nat (_ofs - ofs))) else inr tt)).
+        instantiate (1:=((blk, 0%Z) |-> (List.repeat (Vint 0) sz))).
+        instantiate (1:= echo_black x (z :: ns) ⋅ echo_white x (z :: ns)).
+        eapply URA.auth_update. rr. ii. des; ss. destruct ctx; ss; clarify.
+      }
+      iUpdate SIM.
+      unfold interp_hCallE_tgt, APC. steps. (********** TODO: never unfold it, make a lemma ******************)
+      force_l. exists 0. steps.
+
+      force_l. eexists.
+      hret_tac (@URA.unit Σ) (@URA.unit Σ).
+      { split; try refl; iRefresh. eexists; iRefresh. iSplitP; ss. }
+
+      { split; eauto. iRefresh. iSplitL PRE; eauto. rr. f_equal.
+        rewrite <- Z.negb_odd. rewrite negb_if. des_ifs. }
+      { unfold wf. esplits; eauto. }
+      rewrite unfold_APC. steps.
+
+
+      assert (x = Z.odd n); subst.
+      { hexploit bw_ra_merge; et. intro T. iSpecialize T SIM. iSpecialize T PRE. iPure T. auto. }
+      unfold body_to_tgt. unfold interp_hCallE_tgt, APC. steps. (********** TODO: never unfold it, make a lemma ******************)
+      force_l. exists 0. steps. rewrite unfold_APC. steps.
+      rewrite Any.upcast_downcast. force_l. eexists.
+      hret_tac SIM PRE.
+      { split; eauto. iRefresh. iSplitL PRE; eauto. rr. f_equal.
+        rewrite <- Z.negb_odd. rewrite negb_if. des_ifs. }
+      { unfold wf. esplits; eauto. }
+    }
+
+
+
+
+    { unfold allocF. init. harg_tac. des; clarify.
+      unfold interp_hCallE_tgt, APC. steps. anytac. ss.
+      steps. force_l. exists 0. steps. force_l. exists (Vptr (Mem.nb mem_tgt) 0).
+      set (blk := (Mem.nb mem_tgt)). rename x into sz.
+      assert(WFA: forall ofs, mem_src (Mem.nb mem_tgt) ofs = inr tt).
+      { i.
+        destruct (mem_src (Mem.nb mem_tgt) ofs) eqn:A; cycle 1.
+        { des_u; ss. }
+        destruct o.
+        - admit "ez - add tgt wf".
+        - admit "ez - inl None is boom in RA.excl".
+      }
+      hret_tac (GRA.embed (add_delta_to_black
+                               (URA.black (mem_src: URA.car (t:=Mem1._memRA)))
+                               (points_to (blk, 0%Z) (repeat (Vint 0) sz)): URA.car (t:=Mem1.memRA)))
+      (GRA.embed ((blk, 0%Z) |-> (List.repeat (Vint 0) sz))).
+      { Local Opaque URA.add. etrans.
+        { eapply URA.extends_updatable. eexists; et. }
+        erewrite GRA.embed_add. eapply GRA.embed_updatable.
+        ss. des_ifs. eapply URA.auth_alloc2.
+        eapply URA.wf_mon in VALID.
+        eapply GRA.embed_wf in VALID. des.
+        clear - VALID WFA Heq SIM.
+        Local Transparent URA.add points_to.
+        ss. des. unfold URA.white in Heq. clarify.
+        ii. des_ifs; ss.
+        - bsimpl; des; des_sumbool; clarify.
+          exploit WFA; et. intro A. rewrite A in *; ss.
+        - specialize (VALID0 k k0). bsimpl; des; des_sumbool; clarify; des_ifs.
+        - specialize (VALID0 k k0). bsimpl; des; des_sumbool; clarify; des_ifs.
+          apply_all_once Z.leb_le. apply_all_once Z.ltb_lt.
+          intro A. apply nth_error_None in A. rewrite repeat_length in *.
+          apply inj_le in A. rewrite Z2Nat.id in A; cycle 1.
+          { lia. }
+          lia.
+          Local Opaque URA.add points_to.
+      }
+      { esplits; ss. }
+      { Local Opaque URA.wf.
+        Local Opaque URA.add points_to.
+        Local Transparent points_to.
+        ss. esplits; ss. i. ss.
+        destruct (dec b blk).
+        + subst. unfold blk. unfold update. des_ifs_safe. ss.
+          des_ifs.
+          * bsimpl; des; try rewrite Z.leb_le in *; try rewrite Z.ltb_lt in *.
+            Local Transparent URA.add.
+            s.
+            Local Opaque URA.add.
+            des_ifs; bsimpl; des; des_sumbool; ss; clarify; try rewrite Z.leb_le in *; try rewrite Z.ltb_lt in *;
+              try rewrite Z.leb_gt in *; try rewrite Z.ltb_ge in *; try lia; et.
+            { exploit WFA; et. intro A. rewrite A in *; ss. }
+            { exploit WFA; et. intro A. rewrite A in *; ss. }
+            { rewrite Z.sub_0_r.
+              destruct (nth_error (repeat (Vint 0) sz) (Z.to_nat ofs)) eqn:U.
+              - eapply nth_error_In in U. eapply repeat_spec in U. subst. econs; et.
+              - eapply nth_error_None in U. lia.
+            }
+            { rewrite repeat_length in *. lia. }
+          * Local Transparent URA.add.
+            s.
+            Local Opaque URA.add.
+            des_ifs; bsimpl; des; des_sumbool; ss; clarify; try rewrite Z.leb_le in *; try rewrite Z.ltb_lt in *;
+              try rewrite Z.leb_gt in *; try rewrite Z.ltb_ge in *; try lia; et;
+                try (by exploit WFA; et; intro A; rewrite A in *; ss).
+            { rewrite Z.sub_0_r. rewrite repeat_length in *. lia. }
+            { econs; eauto. }
+            { econs; eauto. }
+        + Local Transparent URA.add.
+          ss.
+          hexploit (SIM b ofs); et. intro A. inv A.
+          {
+            des_ifs; bsimpl; des; des_sumbool; clarify.
+            - unfold update. des_ifs. rewrite <- H1. econs.
+            - unfold update. des_ifs. rewrite <- H1. econs.
+            - unfold update. des_ifs. rewrite <- H1. econs.
+          }
+          {
+            des_ifs; bsimpl; des; des_sumbool; clarify.
+            - unfold update. des_ifs. rewrite <- H1. econs.
+            - unfold update. des_ifs. rewrite <- H1. econs.
+            - unfold update. des_ifs. rewrite <- H1. econs.
+          }
+      }
+    }
+    econs; ss.
+    { unfold freeF. init. harg_tac. des; clarify.
+      unfold interp_hCallE_tgt, APC. steps. anytac. ss.
+      steps. force_l. exists 0. steps. anytac. ss. steps.
+      rewrite URA.unit_idl in *. rewrite GRA.embed_add in *. eapply GRA.embed_wf in VALID. des.
+      rename n into b. rename z into ofs.
+      assert(A: mem_src b ofs = inl (Some v)).
+      { Local Transparent URA.wf.
+        ss.
+        Local Transparent URA.add.
+        ss. des_ifs. des. specialize (VALID0 b ofs).
+        Local Transparent URA.add.
+        clear SIM.
+        Local Transparent URA.unit.
+        ss. clarify. rr in VALID. des. clarify. ss.
+        des_ifs;
+          bsimpl; des; des_sumbool; ss;
+          repeat des_u;
+          clear_tac;
+          try rewrite Z.leb_le in *; try rewrite Z.leb_gt in *; try rewrite Z.ltb_lt in *; try rewrite Z.ltb_ge in *;
+          try rewrite Z.sub_diag in *;
+          try lia; ss.
+        Local Opaque URA.wf URA.add URA.unit.
+      }
+
+      set (mem_src' := fun _b _ofs => if dec _b b && dec _ofs ofs then inr () else mem_src _b _ofs).
+      assert(WF': URA.wf (mem_src': URA.car (t:=Mem1._memRA))).
+      { Local Transparent URA.add URA.wf.
+        ss. ii. des_ifs.
+        ss. clarify.
+        subst mem_src'. ss. des_ifs. des. specialize (VALID0 k k0). bsimpl. des; des_sumbool; des_ifs.
+        Local Opaque URA.wf URA.add.
+      }
+      hexploit (SIM b ofs); et. intro B. rewrite A in *. inv B.
+      force_r.
+      { exfalso. unfold Mem.free in *. des_ifs. }
+      rename t into mem_tgt'.
+      assert(SIM': forall b ofs, sim_loc (Mem.cnts mem_tgt' b ofs) (mem_src' b ofs)).
+      { i.
+        unfold Mem.free in _UNWRAPU. des_ifs. ss.
+        subst mem_src'. ss.
+        destruct (classic (b = b0 /\ ofs = ofs0)); des; clarify.
+        - destruct H0; clarify. (**** TODO: FIX ****) unfold update. des_ifs. econs.
+        - des_ifs.
+          { Psimpl. bsimpl; des; des_sumbool; ss; clarify. destruct H0; ss. destruct H1; ss. (**** TODO: FIX ****)}
+          replace (update (Mem.cnts mem_tgt) b (update (Mem.cnts mem_tgt b) ofs None) b0 ofs0) with
+              (Mem.cnts mem_tgt b0 ofs0); cycle 1.
+          { unfold update. des_ifs. Psimpl. des_ifs; bsimpl; des; des_sumbool; ss; clarify. }
+          et.
+      }
+      force_l. esplits. steps.
+      hret_tac (GRA.embed (URA.black (mem_src': URA.car (t:=Mem1._memRA)))) (@URA.unit Σ).
+      { rewrite URA.unit_id.
+        rewrite ! GRA.embed_add. apply GRA.embed_updatable.
+        apply URA.auth_dealloc.
+        clear - WF' VALID.
+        r. i. rewrite URA.unit_idl.
+        ss. destruct H; clear H. (*** coq bug; des infloops ***) des. clarify.
+        esplits; et.
+        apply func_ext. intro _b. apply func_ext. intro _ofs.
+        destruct (classic (b = _b /\ ofs = _ofs)).
+        - destruct H; clear H. clarify.
+          subst mem_src'. ss. des_ifs; bsimpl; des; des_sumbool; clarify.
+          clear - H0.
+          Local Transparent URA.wf.
+          Local Transparent URA.add.
+          specialize (H0 _b _ofs). ss.
+          des_ifs; bsimpl; des; des_sumbool;
+            try rewrite Z.leb_le in *; try rewrite Z.leb_gt in *; try rewrite Z.ltb_lt in *; try rewrite Z.ltb_ge in *;
+              try rewrite Z.sub_diag in *;
+              try lia; ss.
+          des_u. ss.
+        - Psimpl.
+          subst mem_src'. s.
+          des_ifs; bsimpl; des; des_sumbool;
+            try rewrite Z.leb_le in *; try rewrite Z.leb_gt in *; try rewrite Z.ltb_lt in *; try rewrite Z.ltb_ge in *;
+              try rewrite Z.sub_diag in *;
+              try lia; ss.
+          Local Opaque URA.wf.
+          Local Opaque URA.add.
+      }
+      { split; ss. }
+      { unfold wf. esplits; eauto. }
+    }
+    econs; ss.
+    { unfold loadF. init. harg_tac. des; clarify.
+      unfold interp_hCallE_tgt, APC. steps. anytac. ss.
+      steps. force_l. exists 0. steps. anytac. ss. steps.
+      rewrite URA.unit_idl in *. rewrite GRA.embed_add in *. apply_all_once GRA.embed_wf. des.
+      rename n into b. rename z into ofs.
+      assert(T: mem_src b ofs = inl (Some v)).
+      { Local Transparent points_to URA.add URA.wf URA.unit.
+        clear - VALID.
+        ss. des. do 2 spc VALID0. rr in VALID. des. ss.
+        des_ifs; bsimpl; des; des_sumbool; ss;
+          try rewrite Z.leb_le in *; try rewrite Z.leb_gt in *; try rewrite Z.ltb_lt in *; try rewrite Z.ltb_ge in *;
+            try rewrite Z.sub_diag in *; try lia; ss.
+        Local Opaque points_to URA.add URA.wf URA.unit.
+      }
+      exploit SIM; et. intro U. rewrite T in U. inv U; ss. unfold Mem.load.
+      force_r; ss. clarify. steps. force_l. esplits.
+      hret_tac (GRA.embed (URA.black (mem_src: URA.car (t:=Mem1._memRA)))) (GRA.embed ((b, ofs) |-> [v0])); ss.
+      esplits; eauto.
+    }
+    econs; ss.
+    { unfold storeF. init. harg_tac. des; clarify.
+      unfold interp_hCallE_tgt, APC. steps. anytac. ss.
+      steps. force_l. exists 0. steps. anytac. ss. steps.
+      rewrite URA.unit_idl in *. rewrite GRA.embed_add in *. apply_all_once GRA.embed_wf. des.
+      rename n into b. rename z into ofs.
+      set (mem_src' := fun _b _ofs => if dec _b b && dec _ofs ofs then inl (Some v) else mem_src _b _ofs).
+      assert(WF0: URA.wf (mem_src': URA.car (t:=Mem1._memRA))).
+      { Local Transparent URA.wf.
+        clear - VALID. apply URA.wf_mon in VALID. ss. des.
+        ii. specialize (VALID0 k k0). des_ifs_safe. unfold mem_src' in *. des_ifs.
+        Local Opaque URA.wf.
+      }
+      assert(U: mem_src b ofs = inl (Some v_old)).
+      { Local Transparent URA.add GRA.to_URA points_to URA.wf URA.unit.
+        clear - VALID. ss. des. specialize (VALID0 b ofs). r in VALID. des; clarify. ss.
+        des_ifs; bsimpl; des; des_sumbool; ss; subst;
+          try rewrite Z.leb_le in *; try rewrite Z.leb_gt in *; try rewrite Z.ltb_lt in *; try rewrite Z.ltb_ge in *;
+            try rewrite Z.sub_diag in *; try lia; ss.
+        Local Opaque URA.add GRA.to_URA points_to URA.wf URA.unit.
+      }
+      hexploit SIM; et. intro V. rewrite U in V. inv V; ss. unfold Mem.store. rewrite <- H1. steps.
+      force_l. esplit.
+      hret_tac (GRA.embed (URA.black (mem_src': URA.car (t:=Mem1._memRA)))) (GRA.embed ((b, ofs) |-> [v])).
+      { rewrite ! GRA.embed_add. eapply GRA.embed_updatable.
+        clear - VALID WF0. clear VALID.
+        Local Transparent URA.add GRA.to_URA points_to URA.wf URA.unit.
+        eapply URA.auth_update; et.
+        rr. ii. destruct H; clear H. (*** FIXME: des runs infloop ***)
+        des. subst. esplits; et.
+        subst mem_src'. do 2 (apply func_ext; i). specialize (H0 x x0). specialize (WF0 x x0). ss.
+        des_ifs; bsimpl; des; des_sumbool; ss; subst;
+          try rewrite Z.leb_le in *; try rewrite Z.leb_gt in *; try rewrite Z.ltb_lt in *; try rewrite Z.ltb_ge in *;
+            try rewrite Z.sub_diag in *; try lia; ss.
+        Local Opaque URA.add GRA.to_URA points_to URA.wf URA.unit.
+      }
+      { splits; eauto. }
+      { unfold wf. esplits; eauto. esplits; ss; et. des_ifs.
+        - bsimpl; des; des_sumbool; ss; subst. unfold mem_src'. des_ifs; bsimpl; des; des_sumbool; ss. econs; et.
+        - unfold mem_src'. des_ifs. bsimpl; des; des_sumbool; subst; ss.
+      }
+    }
+    econs; ss.
+    { unfold cmpF. init. harg_tac. unfold interp_hCallE_tgt, APC. steps.
+      destruct PRE as [[? []] ?]. subst.
+      set (resource := c).
+      assert (VALIDPTR: forall b ofs v (WF: URA.wf ((URA.black (mem_src: URA.car (t:=Mem1._memRA))) ⋅ ((b, ofs) |-> [v]))),
+                 Mem.valid_ptr mem_tgt b ofs = true).
+      { clear - SIM. i. cut (mem_src b ofs = inl (Some v)).
+        - i. unfold Mem.valid_ptr.
+          specialize (SIM b ofs). rewrite H in *. inv SIM. ss.
+        - Local Transparent points_to URA.add URA.wf URA.unit.
+          ss. des. specialize (WF0 b ofs). r in WF. des; clarify. ss.
+          des_ifs; bsimpl; des; des_sumbool; ss; subst;
+            try rewrite Z.leb_le in *; try rewrite Z.leb_gt in *; try rewrite Z.ltb_lt in *; try rewrite Z.ltb_ge in *;
+              try rewrite Z.sub_diag in *; try lia; ss.
+          Local Opaque URA.add GRA.to_URA points_to URA.wf URA.unit.
+      }
+      force_l. exists 0. steps. force_l. exists (if b then Vint 1 else Vint 0). des; clarify.
+      - anytac. ss. steps.
+        rewrite URA.unit_idl in *. rewrite GRA.embed_add in *. apply_all_once GRA.embed_wf. des.
+        erewrite VALIDPTR; cycle 1.
+        { instantiate (1:=v). eapply VALID. }
+        steps. hret_tac (GRA.embed (URA.black (mem_src: URA.car (t:=Mem1._memRA)))) resource; ss.
+        esplits; eauto.
+      - anytac. ss. steps.
+        rewrite URA.unit_idl in *. rewrite GRA.embed_add in *. apply_all_once GRA.embed_wf. des.
+        erewrite VALIDPTR; cycle 1.
+        { instantiate (1:=v). eapply VALID. }
+        steps. hret_tac (GRA.embed (URA.black (mem_src: URA.car (t:=Mem1._memRA)))) resource; ss.
+        esplits; eauto.
+      - anytac. ss. steps.
+        rewrite URA.unit_idl in *. repeat rewrite GRA.embed_add in *. apply_all_once GRA.embed_wf. des.
+        erewrite VALIDPTR; cycle 1.
+        { instantiate (1:=v0). clear - VALID.
+          eapply URA.wf_mon. erewrite <- URA.add_assoc. eapply VALID. }
+        erewrite VALIDPTR; cycle 1.
+        { instantiate (1:=v1). clear - VALID.
+          eapply URA.wf_mon. erewrite <- URA.add_assoc.
+          erewrite URA.add_comm with (a:=(b1, ofs1) |-> [v1]). eapply VALID. }
+        ss. destruct (dec b0 b1); cycle 1.
+        { ss. steps. hret_tac (GRA.embed (URA.black (mem_src: URA.car (t:=Mem1._memRA)))) resource; ss.
+          esplits; eauto. }
+        destruct (dec ofs0 ofs1); cycle 1.
+        { ss. steps. hret_tac (GRA.embed (URA.black (mem_src: URA.car (t:=Mem1._memRA)))) resource; ss.
+          esplits; eauto. }
+        subst. exfalso.
+        erewrite URA.add_comm in VALID. eapply URA.wf_mon in VALID.
+        Local Transparent points_to URA.add URA.wf URA.unit.
+        ss. specialize (VALID b1 ofs1).
+        destruct (dec b1 b1); ss. erewrite Z.leb_refl in *. ss.
+        replace (ofs1 <? ofs1 + 1)%Z with true in *; ss.
+        clear. symmetry. eapply Z.ltb_lt. lia.
+        Local Opaque URA.add GRA.to_URA points_to URA.wf URA.unit.
+      - anytac. ss. steps.
+        rewrite URA.unit_idl in *. rewrite GRA.embed_add in *. apply_all_once GRA.embed_wf. des.
+        erewrite VALIDPTR; cycle 1.
+        { instantiate (1:=v). eapply VALID. }
+        ss. destruct (dec b0 b0); ss. destruct (dec ofs ofs); ss. steps.
+        hret_tac (GRA.embed (URA.black (mem_src: URA.car (t:=Mem1._memRA)))) resource; ss.
+        esplits; eauto.
+      - anytac. ss. steps. rewrite URA.unit_idl in *.
+        hret_tac (GRA.embed (URA.black (mem_src: URA.car (t:=Mem1._memRA)))) resource; ss.
+        esplits; eauto.
+    }
+  Qed.
+
+End SIMMODSEM.
